backend/Cminortyping.v
@@ -449,11 +449,11 @@ Inductive wt_state: state -> Prop :=
         (WT_ENV: wt_env env e)
         (DEF_ENV: def_env f e),
       wt_state (State f s k sp e m)
-  | wt_call_state: forall f args k m
+  | wt_call_state: forall f args k m sz
         (WT_FD: wt_fundef f)
         (WT_ARGS: Val.has_type_list args (funsig f).(sig_args))
         (WT_CONT: wt_cont_call k (funsig f).(sig_res)),
-      wt_state (Callstate f args k m)
+      wt_state (Callstate f args k m sz)
   | wt_return_state: forall v k m tret
         (WT_RES: Val.has_type v (proj_rettype tret))
         (WT_CONT: wt_cont_call k tret),
@@ -632,9 +632,10 @@ Lemma wt_find_funct: forall v fd,
 Proof.
   intros. eapply Genv.find_funct_prop; eauto.
 Qed.
-
+Section ORACLE.
+Variable fn_stack_requirements : ident -> Z.
 Lemma subject_reduction:
-  forall st1 t st2, step ge st1 t st2 ->
+  forall st1 t st2, step fn_stack_requirements ge st1 t st2 ->
   forall (WT: wt_state st1), wt_state st2.
 Proof.
   destruct 1; intros; inv WT.
@@ -652,10 +653,10 @@ Proof.
 - inv WT_STMT. econstructor; eauto.
   eapply wt_find_funct; eauto.
   eapply wt_eval_exprlist; eauto.
-  rewrite H8; eapply call_cont_wt; eauto.
+  rewrite H9; eapply call_cont_wt; eauto.
 - inv WT_STMT. exploit external_call_well_typed; eauto. intros TRES.
   econstructor; eauto using wt_Sskip.
-  destruct optid; auto. apply wt_env_assign; auto. rewrite <- H5; auto.
+  destruct optid; auto. apply wt_env_assign; auto. rewrite <- H6; auto.
   destruct optid; auto. apply def_env_assign; auto.
 - inv WT_STMT. econstructor; eauto. econstructor; eauto.
 - inv WT_STMT. destruct b; econstructor; eauto.
@@ -674,10 +675,10 @@ Proof.
   { constructor. eapply call_cont_wt; eauto. }
   generalize (wt_find_label _ _ lbl _ _ H2 WT_CK).
   rewrite H. intros [WT_STMT' WT_CONT']. econstructor; eauto.
-- inv WT_FD. inversion H1; subst. econstructor; eauto.
+- inv WT_FD. inversion H2; subst. econstructor; eauto.
   constructor; auto.
-  apply wt_env_set_locals. apply wt_env_set_params. rewrite H2; auto.
-  red; intros. apply def_set_locals. destruct H4; auto. left; apply def_set_params; auto.
+  apply wt_env_set_locals. apply wt_env_set_params. rewrite H3; auto.
+  red; intros. apply def_set_locals. destruct H5; auto. left; apply def_set_params; auto.
 - exploit external_call_well_typed; eauto. intros.
   econstructor; eauto.
 - inv WT_CONT. econstructor; eauto using wt_Sskip.
@@ -687,20 +688,20 @@ Proof.
 Qed.
 
 Lemma subject_reduction_star:
-  forall st1 t st2, star step ge st1 t st2 ->
+  forall st1 t st2, star (step fn_stack_requirements) ge st1 t st2 ->
   forall (WT: wt_state st1), wt_state st2.
 Proof.
   induction 1; eauto using subject_reduction.
 Qed.
 
 Lemma wt_initial_state:
-  forall S, initial_state p S -> wt_state S.
+  forall S, initial_state fn_stack_requirements p S -> wt_state S.
 Proof.
   intros. inv H. constructor. eapply Genv.find_funct_ptr_prop; eauto.
   rewrite H3; constructor.
   rewrite H3; constructor.
 Qed.
-
+End ORACLE.
 End SUBJECT_REDUCTION.
 
 (** * Safe expressions *)
