backend/RTLgenproof.v
@@ -359,6 +359,7 @@ Qed.
 
 Section CORRECTNESS.
 
+Variable fn_stack_requirements : ident -> Z.
 Variable prog: CminorSel.program.
 Variable tprog: RTL.program.
 Hypothesis TRANSL: match_prog prog tprog.
@@ -416,7 +417,7 @@ Lemma tr_move_correct:
   forall r1 ns r2 nd cs f sp rs m,
   tr_move f.(fn_code) ns r1 nd r2 ->
   exists rs',
-  star step tge (State cs f sp ns rs m) E0 (State cs f sp nd rs' m) /\
+  star (step fn_stack_requirements) tge (State cs f sp ns rs m) E0 (State cs f sp nd rs' m) /\
   rs'#r2 = rs#r1 /\
   (forall r, r <> r2 -> rs'#r = rs#r).
 Proof.
@@ -474,7 +475,7 @@ Definition transl_expr_prop
     (ME: match_env map e le rs)
     (EXT: Mem.extends m tm),
   exists rs', exists tm',
-     star step tge (State cs f sp ns rs tm) E0 (State cs f sp nd rs' tm')
+     star (step fn_stack_requirements) tge (State cs f sp ns rs tm) E0 (State cs f sp nd rs' tm')
   /\ match_env map (set_optvar dst v e) le rs'
   /\ Val.lessdef v rs'#rd
   /\ (forall r, In r pr -> rs'#r = rs#r)
@@ -488,7 +489,7 @@ Definition transl_exprlist_prop
     (ME: match_env map e le rs)
     (EXT: Mem.extends m tm),
   exists rs', exists tm',
-     star step tge (State cs f sp ns rs tm) E0 (State cs f sp nd rs' tm')
+     star (step fn_stack_requirements) tge (State cs f sp ns rs tm) E0 (State cs f sp nd rs' tm')
   /\ match_env map e le rs'
   /\ Val.lessdef_list vl rs'##rl
   /\ (forall r, In r pr -> rs'#r = rs#r)
@@ -502,7 +503,7 @@ Definition transl_condexpr_prop
     (ME: match_env map e le rs)
     (EXT: Mem.extends m tm),
   exists rs', exists tm',
-     plus step tge (State cs f sp ns rs tm) E0 (State cs f sp (if v then ntrue else nfalse) rs' tm')
+     plus (step fn_stack_requirements) tge (State cs f sp ns rs tm) E0 (State cs f sp (if v then ntrue else nfalse) rs' tm')
   /\ match_env map e le rs'
   /\ (forall r, In r pr -> rs'#r = rs#r)
   /\ Mem.extends m tm'.
@@ -742,6 +743,7 @@ Proof.
 (* Exec *)
   split. eapply star_trans. eexact EX1.
   eapply star_left. eapply exec_Icall; eauto.
+  simpl. eauto.
   simpl. rewrite symbols_preserved. rewrite H. eauto. auto.
   eapply star_left. eapply exec_function_external.
   eapply external_call_symbols_preserved; eauto. apply senv_preserved.
@@ -947,7 +949,7 @@ Definition transl_exitexpr_prop
     (ME: match_env map e le rs)
     (EXT: Mem.extends m tm),
   exists nd, exists rs', exists tm',
-     star step tge (State cs f sp ns rs tm) E0 (State cs f sp nd rs' tm')
+     star (step fn_stack_requirements) tge (State cs f sp ns rs tm) E0 (State cs f sp nd rs' tm')
   /\ nth_error nexits x = Some nd
   /\ match_env map e le rs'
   /\ Mem.extends m tm'.
@@ -1228,13 +1230,13 @@ Inductive match_states: CminorSel.state -> RTL.state -> Prop :=
       match_states (CminorSel.State f s k sp e m)
                    (RTL.State cs tf sp ns rs tm)
   | match_callstate:
-      forall f args targs k m tm cs tf
+      forall f args targs k m tm cs tf sz
         (TF: transl_fundef f = OK tf)
         (MS: match_stacks k cs)
         (LD: Val.lessdef_list args targs)
         (MEXT: Mem.extends m tm),
-      match_states (CminorSel.Callstate f args k m)
-                   (RTL.Callstate cs tf targs tm)
+      match_states (CminorSel.Callstate f args k m sz)
+                   (RTL.Callstate cs tf targs tm sz)
   | match_returnstate:
       forall v tv k m tm cs
         (MS: match_stacks k cs)
@@ -1295,10 +1297,10 @@ Proof.
 Qed.
 
 Theorem transl_step_correct:
-  forall S1 t S2, CminorSel.step ge S1 t S2 ->
+  forall S1 t S2, CminorSel.step fn_stack_requirements ge S1 t S2 ->
   forall R1, match_states S1 R1 ->
   exists R2,
-  (plus RTL.step tge R1 t R2 \/ (star RTL.step tge R1 t R2 /\ lt_state S2 S1))
+  (plus (RTL.step fn_stack_requirements) tge R1 t R2 \/ (star (RTL.step fn_stack_requirements) tge R1 t R2 /\ lt_state S2 S1))
   /\ match_states S2 R2.
 Proof.
   induction 1; intros R1 MSTATE; inv MSTATE.
@@ -1318,13 +1320,14 @@ Proof.
   assert ((fn_code tf)!ncont = Some(Ireturn rret)
           /\ match_stacks k cs).
     inv TK; simpl in H; try contradiction; auto.
-  destruct H1.
+  destruct H2.
   assert (fn_stacksize tf = fn_stackspace f).
     inv TF. auto.
   edestruct Mem.free_parallel_extends as [tm' []]; eauto.
+  edestruct Mem.pop_extends as [tm'' []]; eauto.
   econstructor; split.
   left; apply plus_one. eapply exec_Ireturn. eauto.
-  rewrite H3. eauto.
+  rewrite H4. eauto. eauto.
   constructor; auto.
 
   (* assign *)
@@ -1354,7 +1357,7 @@ Proof.
   econstructor; eauto. constructor.
 
   (* call *)
-  inv TS; inv H.
+  inv TS; inv H; inv H0.
   (* indirect *)
   exploit transl_expr_correct; eauto.
   intros [rs' [tm' [A [B [C [D X]]]]]].
@@ -1363,7 +1366,14 @@ Proof.
   exploit functions_translated; eauto. intros [tf' [P Q]].
   econstructor; split.
   left; eapply plus_right. eapply star_trans. eexact A. eexact E. reflexivity.
-  eapply exec_Icall; eauto. simpl. rewrite J. destruct C. eauto. discriminate P. simpl; auto.
+  eapply exec_Icall; eauto.
+  {
+    destruct H3 as (oo & EQ3 & EQ2). red; rewrite EQ3.
+    rewrite J by (simpl; auto).
+    subst. inv C.
+    rewrite symbols_preserved; eauto.
+  }
+  simpl. rewrite J. destruct C. eauto. discriminate P. simpl; auto.
   apply sig_transl_function; auto.
   traceEq.
   constructor; auto. econstructor; eauto.
@@ -1373,14 +1383,22 @@ Proof.
   exploit functions_translated; eauto. intros [tf' [P Q]].
   econstructor; split.
   left; eapply plus_right. eexact E.
-  eapply exec_Icall; eauto. simpl. rewrite symbols_preserved. rewrite H4.
+  eapply exec_Icall; eauto.
+  {
+    destruct H3 as (o & EQ3 & EQ2). inv EQ3. simpl. reflexivity.
+  }
+
+  simpl. rewrite symbols_preserved. rewrite H5.
     rewrite Genv.find_funct_find_funct_ptr in P. eauto.
   apply sig_transl_function; auto.
   traceEq.
+  replace id0 with id.
   constructor; auto. econstructor; eauto.
-
+  apply Genv.find_invert_symbol in H5.
+  destruct H3 as (o & EQ3 & EQ2). inv EQ3.
+  apply Genv.find_invert_symbol in EQ2. congruence.
   (* tailcall *)
-  inv TS; inv H.
+  inv TS; inv H; inv H0.
   (* indirect *)
   exploit transl_expr_correct; eauto.
   intros [rs' [tm' [A [B [C [D X]]]]]].
@@ -1392,7 +1410,14 @@ Proof.
   edestruct Mem.free_parallel_extends as [tm''' []]; eauto.
   econstructor; split.
   left; eapply plus_right. eapply star_trans. eexact A. eexact E. reflexivity.
-  eapply exec_Itailcall; eauto. simpl. rewrite J. destruct C. eauto. discriminate P. simpl; auto.
+  eapply exec_Itailcall; eauto.
+  {
+    destruct H3 as (oo & EQ3 & EQ2). red; rewrite EQ3.
+    rewrite J by (simpl; auto).
+    subst. inv C.
+    rewrite symbols_preserved; eauto.
+  }
+  simpl. rewrite J. destruct C. eauto. discriminate P. simpl; auto.
   apply sig_transl_function; auto.
   rewrite H; eauto.
   traceEq.
@@ -1406,13 +1431,20 @@ Proof.
   edestruct Mem.free_parallel_extends as [tm''' []]; eauto.
   econstructor; split.
   left; eapply plus_right. eexact E.
-  eapply exec_Itailcall; eauto. simpl. rewrite symbols_preserved. rewrite H5.
+  eapply exec_Itailcall; eauto.
+  {
+    destruct H3 as (o & EQ3 & EQ2). inv EQ3. simpl. reflexivity.
+  }
+  simpl. rewrite symbols_preserved. rewrite H6.
   rewrite Genv.find_funct_find_funct_ptr in P. eauto.
   apply sig_transl_function; auto.
   rewrite H; eauto.
   traceEq.
+  replace id0 with id.
   constructor; auto.
-
+  apply Genv.find_invert_symbol in H6.
+  destruct H3 as (o & EQ3 & EQ2). inv EQ3.
+  apply Genv.find_invert_symbol in EQ2. congruence.
   (* builtin *)
   inv TS.
   exploit invert_eval_builtin_args; eauto. intros (vparams & P & Q).
@@ -1491,11 +1523,12 @@ Proof.
   exploit match_stacks_call_cont; eauto. intros [U V].
   inversion TF.
   edestruct Mem.free_parallel_extends as [tm' []]; eauto.
+  edestruct Mem.pop_extends as [tm'' []]; eauto.
   econstructor; split.
   left; apply plus_one. eapply exec_Ireturn; eauto.
-  rewrite H2; eauto.
+  rewrite H3; eauto.
   constructor; auto.
-
+  
   (* return some *)
   inv TS.
   exploit transl_expr_correct; eauto.
@@ -1503,9 +1536,10 @@ Proof.
   exploit match_stacks_call_cont; eauto. intros [U V].
   inversion TF.
   edestruct Mem.free_parallel_extends as [tm'' []]; eauto.
+  edestruct Mem.pop_extends as [tm''' []]; eauto.
   econstructor; split.
   left; eapply plus_right. eexact A. eapply exec_Ireturn; eauto.
-  rewrite H4; eauto. traceEq.
+  rewrite H5; eauto. traceEq.
   simpl. constructor; auto.
 
   (* label *)
@@ -1539,6 +1573,7 @@ Proof.
   simpl. econstructor; eauto.
   econstructor; eauto.
   inversion MS; subst; econstructor; eauto.
+  apply Mem.push_extends. auto.
 
   (* external call *)
   monadInv TF.
@@ -1557,8 +1592,8 @@ Proof.
 Qed.
 
 Lemma transl_initial_states:
-  forall S, CminorSel.initial_state prog S ->
-  exists R, RTL.initial_state tprog R /\ match_states S R.
+  forall S, CminorSel.initial_state fn_stack_requirements prog S ->
+  exists R, RTL.initial_state fn_stack_requirements tprog R /\ match_states S R.
 Proof.
   induction 1.
   exploit function_ptr_translated; eauto. intros [tf [A B]].
@@ -1568,6 +1603,7 @@ Proof.
   symmetry; eapply match_program_main; eauto.
   eexact A.
   rewrite <- H2. apply sig_transl_function; auto.
+  destruct TRANSL as (_&MAIN&_). setoid_rewrite <- MAIN.
   constructor. auto. constructor.
   constructor. apply Mem.extends_refl.
 Qed.
@@ -1580,7 +1616,8 @@ Proof.
 Qed.
 
 Theorem transf_program_correct:
-  forward_simulation (CminorSel.semantics prog) (RTL.semantics tprog).
+  forward_simulation (CminorSel.semantics fn_stack_requirements prog)
+                     (RTL.semantics fn_stack_requirements tprog).
 Proof.
   eapply forward_simulation_star_wf with (order := lt_state).
   apply senv_preserved.
