backend/Selectionproof.v
@@ -114,6 +114,7 @@ Qed.
 
 Section PRESERVATION.
 
+Variable fn_stack_requirements : ident -> Z.
 Variable prog: Cminor.program.
 Variable tprog: CminorSel.program.
 Let ge := Genv.globalenv prog.
@@ -247,7 +248,8 @@ Lemma eval_store:
   eval_expr tge sp e m nil a1 v1 ->
   eval_expr tge sp e m nil a2 v2 ->
   Mem.storev chunk m v1 v2 = Some m' ->
-  step tge (State f (store chunk a1 a2) k sp e m)
+  step fn_stack_requirements tge
+       (State f (store chunk a1 a2) k sp e m)
         E0 (State f Sskip k sp e m').
 Proof.
   intros. generalize H1; destruct v1; simpl; intro; try discriminate.
@@ -840,41 +842,73 @@ Lemma sel_builtin_res_correct:
 Proof.
   intros. destruct oid; simpl; auto. apply set_var_lessdef; auto.
 Qed.
+Lemma push_exter_pop :forall ef ge vl m1 t v m2,
+    external_call ef ge vl (Mem.push m1) t v m2 ->
+    {m3:mem| Mem.pop m2 = Some m3}.
+Proof.
+  intros.
+  apply Mem.nonempty_pop.
+  apply external_call_mem_stackeq in H. unfold Mem.stack_mem.
+  rewrite <- H. simpl. congruence.
+Qed.
 
+Lemma push_pop : forall m1,
+    Mem.pop (Mem.push m1) = Some m1.
+Proof.
+  intros.
+  destruct (Mem.stack (Mem.support (Mem.push m1))) eqn:Hstk.
+  - simpl in Hstk. congruence.
+  - unfold Mem.pop.
+    rewrite pred_dec_false; eauto.
+    unfold Mem.unchecked_pop. unfold Mem.sup_pop.
+    rewrite Hstk.
+ 
+  destruct (Mem.stack (Mem.support (Mem.push m1))).
 Lemma sel_builtin_default_correct:
   forall optid ef al sp e1 m1 vl t v m2 e1' m1' f k,
   Cminor.eval_exprlist ge sp e1 m1 al vl ->
-  external_call ef ge vl m1 t v m2 ->
+  external_call ef ge vl (Mem.push m1) t v m2 ->
   env_lessdef e1 e1' -> Mem.extends m1 m1' ->
-  exists e2' m2',
-     plus step tge (State f (sel_builtin_default optid ef al) k sp e1' m1')
+  exists e2' m3 m2',
+     plus (step fn_stack_requirements) tge (State f (sel_builtin_default optid ef al) k sp e1' m1')
                  t (State f Sskip k sp e2' m2')
   /\ env_lessdef (set_optvar optid v e1) e2'
-  /\ Mem.extends m2 m2'.
+  /\ Mem.pop m2 = Some m3
+  /\ Mem.extends m3 m2'.
 Proof.
   intros. unfold sel_builtin_default.
   exploit sel_builtin_args_correct; eauto. intros (vl' & A & B).
-  exploit external_call_mem_extends; eauto. intros (v' & m2' & D & E & F & _).
-  econstructor; exists m2'; split.
+  exploit external_call_mem_extends; eauto.
+  eapply Mem.push_extends; eauto.
+  intros (v' & m2' & D & E & F & _).
+  apply push_exter_pop in H0. destruct H0 as[m3 POP1].
+  exploit Mem.pop_extends; eauto.
+  intros (m3' & G & I).
+  econstructor; exists m3; exists m3'; split.
   apply plus_one.
-  econstructor. eexact A. eapply external_call_symbols_preserved. eexact senv_preserved. eexact D.
-  split; auto. apply sel_builtin_res_correct; auto.
-Qed. 
+  econstructor. eexact A. eapply external_call_symbols_preserved. eexact senv_preserved.
+  eexact D. auto.
+  econstructor.
+  apply sel_builtin_res_correct; auto. auto.
+Qed.
 
 Lemma sel_builtin_correct:
   forall optid ef al sp e1 m1 vl t v m2 e1' m1' f k,
   Cminor.eval_exprlist ge sp e1 m1 al vl ->
-  external_call ef ge vl m1 t v m2 ->
+  external_call ef ge vl (Mem.push m1) t v m2 ->
   env_lessdef e1 e1' -> Mem.extends m1 m1' ->
-  exists e2' m2',
-     plus step tge (State f (sel_builtin optid ef al) k sp e1' m1')
+  exists e2' m3 m2',
+     plus (step fn_stack_requirements) tge (State f (sel_builtin optid ef al) k sp e1' m1')
                  t (State f Sskip k sp e2' m2')
   /\ env_lessdef (set_optvar optid v e1) e2'
-  /\ Mem.extends m2 m2'.
+  /\ Mem.pop m2 = Some m3
+  /\ Mem.extends m3 m2'.
 Proof.
-  intros. 
+  intros.
   exploit sel_exprlist_correct; eauto. intros (vl' & A & B).
-  exploit external_call_mem_extends; eauto. intros (v' & m2' & D & E & F & _).
+  exploit external_call_mem_extends; eauto.
+  exploit Mem.push_extends; eauto.
+  intros (v' & m2' & D & E & F & _).
   unfold sel_builtin.
   destruct ef; eauto using sel_builtin_default_correct.
   destruct (lookup_builtin_function name sg) as [bf|] eqn:LKUP; eauto using sel_builtin_default_correct.
@@ -882,12 +916,15 @@ Proof.
   destruct optid as [id|]; eauto using sel_builtin_default_correct.
 - destruct (sel_known_builtin bf (sel_exprlist al)) as [a|] eqn:SKB; eauto using sel_builtin_default_correct.
   exploit eval_sel_known_builtin; eauto. intros (v'' & U & V).
-  econstructor; exists m2'; split.
+  apply push_exter_pop in H0. destruct H0 as[m3 POP1].
+  exploit Mem.pop_extends; eauto.
+  intros (m3' & G & I).
+  econstructor; exists m3; exists m3'; split.
   apply plus_one. econstructor. eexact U.
   split; auto. apply set_var_lessdef; auto. apply Val.lessdef_trans with v'; auto.
 - exists e1', m2'; split.
   eapply plus_two. constructor. constructor. auto.
-  simpl; auto.  
+  simpl; auto.
 Qed.
 
 (** If-conversion *)
@@ -895,7 +932,7 @@ Qed.
 Lemma classify_stmt_sound_1:
   forall f sp e m s k,
   classify_stmt s = SCskip ->
-  star Cminor.step ge (Cminor.State f s k sp e m) E0 (Cminor.State f Cminor.Sskip k sp e m).
+  star (Cminor.step fn_stack_requirements) ge (Cminor.State f s k sp e m) E0 (Cminor.State f Cminor.Sskip k sp e m).
 Proof.
   intros until s; functional induction (classify_stmt s); intros; try discriminate.
   - apply star_refl.
@@ -911,7 +948,7 @@ Lemma classify_stmt_sound_2:
   Cminor.eval_expr ge sp e m a v ->
   forall s k,
   classify_stmt s = SCassign id a ->
-  star Cminor.step ge (Cminor.State f s k sp e m) E0 (Cminor.State f Cminor.Sskip k sp (PTree.set id v e) m).
+  star (Cminor.step fn_stack_requirements) ge (Cminor.State f s k sp e m) E0 (Cminor.State f Cminor.Sskip k sp (PTree.set id v e) m).
 Proof.
   intros until s; functional induction (classify_stmt s); intros; try discriminate.
   - inv H0. apply star_one. constructor; auto.
@@ -976,8 +1013,8 @@ Lemma if_conversion_correct:
   env_lessdef e e' -> Mem.extends m m' ->
   let s0 := if b then ifso else ifnot in
   exists e1 e1',
-     step tge (State f' s k' sp e' m') E0 (State f' Sskip k' sp e1' m')
-  /\ star Cminor.step ge (Cminor.State f s0 k sp e m) E0 (Cminor.State f Cminor.Sskip k sp e1 m)
+     step fn_stack_requirements tge (State f' s k' sp e' m') E0 (State f' Sskip k' sp e1' m')
+  /\ star (Cminor.step fn_stack_requirements) ge (Cminor.State f s0 k sp e m) E0 (Cminor.State f Cminor.Sskip k sp e1 m)
   /\ env_lessdef e1 e1'.
 Proof.
   unfold if_conversion; intros until m'; intros IFC DE WTE WT1 WT2 EVC BOV ELD MEXT.
@@ -1063,15 +1100,15 @@ Inductive match_states: Cminor.state -> CminorSel.state -> Prop :=
       match_states
         (Cminor.State f s k sp e m)
         (State f' s' k' sp e' m')
-  | match_callstate: forall cunit f f' args args' k k' m m'
+  | match_callstate: forall cunit f f' args args' k k' m m' id
         (LINK: linkorder cunit prog)
         (TF: match_fundef cunit f f')
         (MC: match_call_cont k k')
         (LD: Val.lessdef_list args args')
         (ME: Mem.extends m m'),
       match_states
-        (Cminor.Callstate f args k m)
-        (Callstate f' args' k' m')
+        (Cminor.Callstate f args k m id)
+        (Callstate f' args' k' m' id)
   | match_returnstate: forall v v' k k' m m'
         (MC: match_call_cont k k')
         (LD: Val.lessdef v v')
@@ -1079,19 +1116,20 @@ Inductive match_states: Cminor.state -> CminorSel.state -> Prop :=
       match_states
         (Cminor.Returnstate v k m)
         (Returnstate v' k' m')
-  | match_builtin_1: forall cunit hf ef args optid f sp e k m al f' e' k' m' env
+  | match_builtin_1: forall cunit hf ef args optid f sp e k m1 m2 al f' e' k' m' env sz
         (LINK: linkorder cunit prog)
         (HF: helper_functions_declared cunit hf)
         (TF: sel_function (prog_defmap cunit) hf f = OK f')
         (TYF: type_function f = OK env)
         (MC: match_cont cunit hf (known_id f) env k k')
-        (EA: Cminor.eval_exprlist ge sp e m al args)
+        (EA: Cminor.eval_exprlist ge sp e m1 al args)
         (LDE: env_lessdef e e')
-        (ME: Mem.extends m m'),
+        (PUSH: Mem.push m1 = m2)
+        (ME: Mem.extends m1 m'),
       match_states
-        (Cminor.Callstate (External ef) args (Cminor.Kcall optid f sp e k) m)
+        (Cminor.Callstate (External ef) args (Cminor.Kcall optid f sp e k) m2 sz)
         (State f' (sel_builtin optid ef al) k' sp e' m')
-  | match_builtin_2: forall cunit hf v v' optid f sp e k m f' e' m' k' env
+  | match_builtin_2: forall cunit hf v v' optid f sp e k m1 m2 f' e' m' k' env
         (LINK: linkorder cunit prog)
         (HF: helper_functions_declared cunit hf)
         (TF: sel_function (prog_defmap cunit) hf f = OK f')
@@ -1099,9 +1137,10 @@ Inductive match_states: Cminor.state -> CminorSel.state -> Prop :=
         (MC: match_cont cunit hf (known_id f) env k k')
         (LDV: Val.lessdef v v')
         (LDE: env_lessdef (set_optvar optid v e) e')
-        (ME: Mem.extends m m'),
+        (ME: Mem.extends m2 m')
+        (POP: Mem.pop m1 = Some m2),
       match_states
-        (Cminor.Returnstate v (Cminor.Kcall optid f sp e k) m)
+        (Cminor.Returnstate v (Cminor.Kcall optid f sp e k) m1)
         (State f' Sskip k' sp e' m').
 
 Remark call_cont_commut:
@@ -1234,17 +1273,17 @@ Qed.
 
 Definition measure (s: Cminor.state) : nat :=
   match s with
-  | Cminor.Callstate _ _ _ _ => 0%nat
-  | Cminor.State _ _ _ _ _ _ => 1%nat
-  | Cminor.Returnstate _ _ _ => 2%nat
+  | Cminor.Callstate _ _ _ _ _ => 0%nat
+  | Cminor.State _ _ _ _ _ _   => 1%nat
+  | Cminor.Returnstate _ _ _   => 2%nat
   end.
 
 Lemma sel_step_correct:
-  forall S1 t S2, Cminor.step ge S1 t S2 ->
+  forall S1 t S2, Cminor.step fn_stack_requirements ge S1 t S2 ->
   forall T1, match_states S1 T1 -> wt_state S1 ->
-  (exists T2, plus step tge T1 t T2 /\ match_states S2 T2)
+  (exists T2, plus (step fn_stack_requirements) tge T1 t T2 /\ match_states S2 T2)
   \/ (measure S2 < measure S1 /\ t = E0 /\ match_states S2 T1)%nat
-  \/ (exists S3 T2, star Cminor.step ge S2 E0 S3 /\ step tge T1 t T2 /\ match_states S3 T2).
+  \/ (exists S3 T2, star (Cminor.step fn_stack_requirements) ge S2 E0 S3 /\ step fn_stack_requirements tge T1 t T2 /\ match_states S3 T2).
 Proof.
   induction 1; intros T1 ME WTS; inv ME; try (monadInv TS).
 - (* skip seq *)
@@ -1257,7 +1296,7 @@ Proof.
   exploit Mem.free_parallel_extends; eauto. intros [m2' [A B]].
   left; econstructor; split.
   apply plus_one; econstructor. eapply match_is_call_cont; eauto.
-  erewrite stackspace_function_translated; eauto.
+  erewrite stackspace_function_translated; eauto. eauto.
   econstructor; eauto. eapply match_is_call_cont; eauto.
 - (* assign *)
   exploit sel_expr_correct; eauto. intros [v' [A B]].
@@ -1273,29 +1312,41 @@ Proof.
   econstructor; eauto.
 - (* Scall *)
   exploit classify_call_correct; eauto.
-  destruct (classify_call (prog_defmap cunit) a) as [ | id | ef].
+  destruct (classify_call (prog_defmap cunit) a) as [ | id' | ef].
 + (* indirect *)
   exploit sel_expr_correct; eauto. intros [vf' [A B]].
   exploit sel_exprlist_correct; eauto. intros [vargs' [C D]].
   exploit functions_translated; eauto. intros (cunit' & fd' & U & V & W).
   left; econstructor; split.
-  apply plus_one; econstructor; eauto. econstructor; eauto.
+  apply plus_one; econstructor; eauto.
+  destruct H as (bb & oo & EQ & EQ'). subst. inv B.
+  eexists; eexists; split; eauto. rewrite symbols_preserved; eauto.
+  econstructor; eauto.
   eapply sig_function_translated; eauto.
   eapply match_callstate with (cunit := cunit'); eauto.
   eapply match_cont_call with (cunit := cunit) (hf := hf); eauto.
+  eapply Mem.push_extends; eauto.
 + (* direct *)
   intros [b [U V]].
   exploit sel_exprlist_correct; eauto. intros [vargs' [C D]].
   exploit functions_translated; eauto. intros (cunit' & fd' & X & Y & Z).
+  destruct H as (bb & oo & EQ & EQ'). subst. inv V.
   left; econstructor; split.
   apply plus_one; econstructor; eauto.
-  subst vf. econstructor; eauto. rewrite symbols_preserved; eauto.
+  econstructor; eauto. rewrite symbols_preserved; eauto.
+  econstructor; eauto. rewrite symbols_preserved; eauto.
   eapply sig_function_translated; eauto.
+  replace id' with id.
   eapply match_callstate with (cunit := cunit'); eauto.
   eapply match_cont_call with (cunit := cunit) (hf := hf); eauto.
+  eapply Mem.push_extends; eauto.
+  apply Genv.find_invert_symbol in U.
+  apply Genv.find_invert_symbol in EQ'.
+  congruence.
 + (* turned into Sbuiltin *)
   intros EQ. subst fd.
   right; left; split. simpl; lia. split; auto. econstructor; eauto.
+  
 - (* Stailcall *)
   exploit Mem.free_parallel_extends; eauto. intros [m2' [P Q]].
   erewrite <- stackspace_function_translated in P by eauto.
@@ -1305,11 +1356,20 @@ Proof.
   left; econstructor; split.
   apply plus_one.
   exploit classify_call_correct. eexact LINK. eauto. eauto.
-  destruct (classify_call (prog_defmap cunit)) as [ | id | ef]; intros.
-  econstructor; eauto. econstructor; eauto. eapply sig_function_translated; eauto.
-  destruct H2 as [b [U V]]. subst vf. inv B.
-  econstructor; eauto. econstructor; eauto. rewrite symbols_preserved; eauto. eapply sig_function_translated; eauto.
-  econstructor; eauto. econstructor; eauto. eapply sig_function_translated; eauto.
+  destruct (classify_call (prog_defmap cunit)) as [ | id' | ef]; intros.
+  econstructor; eauto.
+  destruct H as (bb & oo & EQ & EQ'). subst. inv B.
+  eexists; eexists; split; eauto. rewrite symbols_preserved; eauto.
+  econstructor; eauto. eapply sig_function_translated; eauto.
+  destruct H3 as [b [U V]]. subst vf. inv B.
+  econstructor; eauto.
+  destruct H as (bb & oo & EQ & EQ'). inv EQ. subst.
+  eexists; eexists; split; eauto. rewrite symbols_preserved; eauto.
+  econstructor; eauto. rewrite symbols_preserved; eauto. eapply sig_function_translated; eauto.
+  econstructor; eauto.
+  destruct H as (bb & oo & EQ & EQ'). subst. inv B.
+  eexists; eexists; split; eauto. rewrite symbols_preserved; eauto.
+  econstructor; eauto. eapply sig_function_translated; eauto.
   eapply match_callstate with (cunit := cunit'); eauto.
   eapply call_cont_commut; eauto.
 - (* Sbuiltin *)
@@ -1364,6 +1424,7 @@ Proof.
   erewrite <- stackspace_function_translated in P by eauto.
   left; econstructor; split.
   apply plus_one; econstructor. simpl; eauto.
+  eauto.
   econstructor; eauto. eapply call_cont_commut; eauto.
 - (* Sreturn Some *)
   exploit Mem.free_parallel_extends; eauto. intros [m2' [P Q]].
@@ -1387,10 +1448,11 @@ Proof.
   apply plus_one; econstructor; eauto.
   econstructor; eauto.
 - (* internal function *)
-  destruct TF as (hf & HF & TF). 
+  destruct TF as (hf & HF & TF).
   monadInv TF. generalize EQ; intros TF; monadInv TF.
   exploit Mem.alloc_extends. eauto. eauto. apply Z.le_refl. apply Z.le_refl.
   intros [m2' [A B]].
+  exploit Mem.record_extends; eauto. intros [m2''[A' B']].
   left; econstructor; split.
   apply plus_one; econstructor; simpl; eauto.
   econstructor; simpl; eauto.
@@ -1404,21 +1466,24 @@ Proof.
   left; econstructor; split.
   apply plus_one; econstructor. eapply external_call_symbols_preserved; eauto. apply senv_preserved.
   econstructor; eauto.
-- (* external call turned into a Sbuiltin *)
-  exploit sel_builtin_correct; eauto. intros (e2' & m2' & P & Q & R).
-  left; econstructor; split. eexact P. econstructor; eauto.
+-  (* external call turned into a Sbuiltin *)
+  
+(*  exploit sel_builtin_correct; eauto. intros (e2' & m2' & P & Q & R). *)
+  left; econstructor; split. Check sel_builtin_correct.
+
+ eexact P. econstructor; eauto.
 - (* return *)
   inv MC.
   left; econstructor; split.
-  apply plus_one; econstructor.
+  apply plus_one; econstructor. eauto.
   econstructor; eauto. destruct optid; simpl; auto. apply set_var_lessdef; auto.
 - (* return of an external call turned into a Sbuiltin *)
   right; left; split. simpl; lia. split. auto. econstructor; eauto.
 Qed.
 
 Lemma sel_initial_states:
-  forall S, Cminor.initial_state prog S ->
-  exists R, initial_state tprog R /\ match_states S R.
+  forall S, Cminor.initial_state fn_stack_requirements prog S ->
+  exists R, initial_state fn_stack_requirements tprog R /\ match_states S R.
 Proof.
   destruct 1.
   exploit function_ptr_translated; eauto. intros (cu & f' & A & B & C).
@@ -1428,7 +1493,8 @@ Proof.
   rewrite (match_program_main TRANSF). fold tge. rewrite symbols_preserved. eauto.
   eexact A.
   rewrite <- H2. eapply sig_function_translated; eauto.
-  econstructor; eauto. constructor. apply Mem.extends_refl.
+  destruct TRANSF as (_ & MAIN & _); rewrite MAIN. econstructor; eauto.
+  constructor. apply Mem.extends_refl.
 Qed.
 
 Lemma sel_final_states:
@@ -1439,17 +1505,17 @@ Proof.
 Qed.
 
 Theorem transf_program_correct:
-  forward_simulation (Cminor.semantics prog) (CminorSel.semantics tprog).
+  forward_simulation (Cminor.semantics fn_stack_requirements prog) (CminorSel.semantics fn_stack_requirements tprog).
 Proof.
   set (MS := fun S T => match_states S T /\ wt_state S).
   apply forward_simulation_determ_star with (match_states := MS) (measure := measure).
 - apply Cminor.semantics_determinate.
 - apply senv_preserved.
-- intros. exploit sel_initial_states; eauto. intros (T & P & Q). 
-  exists T; split; auto; split; auto. eapply wt_initial_state. eexact wt_prog. auto. 
+- intros. exploit sel_initial_states; eauto. intros (T & P & Q).
+  exists T; split; auto; split; auto. eapply wt_initial_state. eexact wt_prog. apply H.
 - intros. destruct H. eapply sel_final_states; eauto.
 - intros S1 t S2 A T1 [B C].
-  assert (wt_state S2) by (eapply subject_reduction; eauto using wt_prog).
+  assert (wt_state S2). { eapply subject_reduction; eauto using wt_prog. apply A. }
   unfold MS.
   exploit sel_step_correct; eauto.
   intros [(T2 & D & E) | [(D & E & F) | (S3 & T2 & D & E & F)]].
